checker for the new invariants

pulse/src/checker/Pulse.Checker.WithInv.fst
@@ -44,79 +44,74 @@ let rt_recheck (gg:env) (#g:T.env) (#e:T.term) (#ty: T.typ) () : T.Tac (RT.tot_t
 let recheck (#g:env) (#e:term) (#ty: typ) () : T.Tac (tot_typing g e ty) =
   core_check_tot_term g e ty
 
-let term_remove_inv (inv:vprop) (tm:term) : T.Tac (tm':term { tm_star tm' inv == tm}) =
-  match inspect_term tm with
-  | Tm_Star tm inv' ->
-    if eq_tm inv inv' then tm
-    else T.fail "term_remove_inv"
-  | _ ->
-    T.fail "term_remove_inv: not a star?"
+// let term_remove_inv (inv:vprop) (tm:term) : T.Tac (tm':term { tm_star tm' inv == tm}) =
+//   match inspect_term tm with
+//   | Tm_Star tm inv' ->
+//     if eq_tm inv inv' then tm
+//     else T.fail "term_remove_inv"
+//   | _ ->
+//     T.fail "term_remove_inv: not a star?"
 
-let st_comp_remove_inv (inv:vprop) (c:st_comp) : T.Tac (s:st_comp { add_frame (C_ST s) inv == (C_ST c) }) =
-  { c with pre = term_remove_inv inv c.pre
-         ; post = term_remove_inv inv c.post }
+// let st_comp_remove_inv (inv:vprop) (c:st_comp) : T.Tac (s:st_comp { add_frame (C_ST s) inv == (C_ST c) }) =
+//   { c with pre = term_remove_inv inv c.pre
+//          ; post = term_remove_inv inv c.post }
 
-#push-options "--z3rlimit 50 --query_stats --split_queries no --max_fuel 2 --max_ifuel 1"  
-let check_iname_disjoint (g:env) (r:range) (inv_p inames inv:term)
-: T.Tac (Pulse.Typing.prop_validity g (inv_disjointness inv_p inames inv))
-= let goal = inv_disjointness inv_p inames inv in
-  let (| tag, goal_typing |) =
-    Pulse.Checker.Pure.core_check_term_at_type g goal tm_prop
-  in
-  if tag <> T.E_Total
-  then T.fail "Impossible: prop typing is always total"
-  else (
-    let tok = Pulse.Checker.Pure.try_check_prop_validity g goal goal_typing in
-    match tok with
-    | None ->
-      fail_doc g (Some r) [
-        Pulse.PP.text "Failed to prove that an invariant is not recursively opened:";
-        Pulse.PP.prefix 4 1 (Pulse.PP.text "The set of invariant names: ") (Pulse.PP.pp inames);
-        Pulse.PP.prefix 4 1 (Pulse.PP.text "may contain the invariant: ") (Pulse.PP.pp inv);
-      ]
-    | Some tok -> tok
-  )
- 
-#push-options "--ifuel 2 --fuel 8"
-let remove_iname (inv_p inames inv:term)
+// #push-options "--z3rlimit 50 --query_stats --split_queries no --max_fuel 2 --max_ifuel 1"  
+// let check_iname_disjoint (g:env) (r:range) (inv_p inames inv:term)
+// : T.Tac (Pulse.Typing.prop_validity g (inv_disjointness inv_p inames inv))
+// = let goal = inv_disjointness inv_p inames inv in
+//   let (| tag, goal_typing |) =
+//     Pulse.Checker.Pure.core_check_term_at_type g goal tm_prop
+//   in
+//   if tag <> T.E_Total
+//   then T.fail "Impossible: prop typing is always total"
+//   else (
+//     let tok = Pulse.Checker.Pure.try_check_prop_validity g goal goal_typing in
+//     match tok with
+//     | None ->
+//       fail_doc g (Some r) [
+//         Pulse.PP.text "Failed to prove that an invariant is not recursively opened:";
+//         Pulse.PP.prefix 4 1 (Pulse.PP.text "The set of invariant names: ") (Pulse.PP.pp inames);
+//         Pulse.PP.prefix 4 1 (Pulse.PP.text "may contain the invariant: ") (Pulse.PP.pp inv);
+//       ]
+//     | Some tok -> tok
+//   )
+
+let remove_iname (inames i:term)
 : term
 = wr 
     (Pulse.Reflection.Util.remove_inv_tm
-      (elab_term inv_p)
       (elab_term inames)
-      (elab_term inv))
+      (elab_term i))
   (Pulse.RuntimeUtils.range_of_term inames)
-let add_iname (inv_p inames inv:term)
+
+let add_iname (inames i:term)
 : term
 = wr 
     (Pulse.Reflection.Util.add_inv_tm
-      (elab_term inv_p)
       (elab_term inames)
-      (elab_term inv))
+      (elab_term i))
   (Pulse.RuntimeUtils.range_of_term inames)
-#pop-options
 
 module RU = Pulse.RuntimeUtils
 let all_inames =
-  wr Pulse.Reflection.Util.all_inames_tm FStar.Range.range_0
+  wr Pulse.Syntax.Pure.tm_all_inames FStar.Range.range_0
 let all_inames_typing (g:env)
 : tot_typing g all_inames tm_inames
 = RU.magic()
 
 let remove_iname_typing
-    (g:env) (#inv_p #inames #inv:term)
-    (_:tot_typing g inv_p tm_vprop)
+    (g:env) (#inames #i:term)
     (_:tot_typing g inames tm_inames)
-    (_:tot_typing g inv (tm_inv inv_p))
-: tot_typing g (remove_iname inv_p inames inv) tm_inames
+    (_:tot_typing g i tm_iname_ref)
+: tot_typing g (remove_iname inames i) tm_inames
 = RU.magic()
 
 let add_iname_typing
-    (g:env) (#inv_p #inames #inv:term)
-    (_:tot_typing g inv_p tm_vprop)
+    (g:env) (#inames #i:term)
     (_:tot_typing g inames tm_inames)
-    (_:tot_typing g inv (tm_inv inv_p))
-: tot_typing g (add_iname inv_p inames inv) tm_inames
+    (_:tot_typing g i tm_iname_ref)
+: tot_typing g (add_iname inames i) tm_inames
 = RU.magic()
 
 let tm_inames_subset_typing
@@ -126,33 +121,26 @@ let tm_inames_subset_typing
 : tot_typing g (tm_inames_subset i j) tm_prop
 = RU.magic()
 
-let disjointness_remove_i_i (g:env) (inv_p inames inv:term)
-: T.Tac (Pulse.Typing.prop_validity g 
-            (inv_disjointness inv_p (remove_iname inv_p inames inv) inv))
+let disjointness_remove_i_i (g:env) (inames i:term)
+: T.Tac (Pulse.Typing.prop_validity g (inv_disjointness (remove_iname inames i) i))
 = RU.magic()
 
 let add_remove_inverse (g:env)
-     (inv_p inames inv:term)
-     (inv_p_typing:tot_typing g inv_p tm_vprop)
+     (inames i:term)
      (inames_typing:tot_typing g inames tm_inames)
-     (inv_typing:tot_typing g inv (tm_inv inv_p))
+     (i_typing:tot_typing g i tm_iname_ref)
 : T.Tac 
-    (prop_validity g 
-        (tm_inames_subset 
-            (add_iname inv_p
-              (remove_iname inv_p inames inv)
-              inv)
-            inames))
+    (prop_validity g (tm_inames_subset (add_iname (remove_iname inames i) i) inames))
 = let typing
   : tot_typing g 
           (tm_inames_subset 
-              (add_iname inv_p
-                (remove_iname inv_p inames inv)
-                inv)
+              (add_iname
+                (remove_iname inames i)
+                i)
               inames)
           tm_prop
-  = let remove_typing = remove_iname_typing g inv_p_typing inames_typing inv_typing in
-    let add_typing = add_iname_typing g inv_p_typing remove_typing inv_typing in
+  = let remove_typing = remove_iname_typing g inames_typing i_typing in
+    let add_typing = add_iname_typing g remove_typing i_typing in
     tm_inames_subset_typing g 
       add_typing
       inames_typing
@@ -163,27 +151,121 @@ let add_remove_inverse (g:env)
     fail_doc g None [
       Pulse.PP.text "Failed to prove that only the following invariants are opened";
       prefix 4 1 (text "Inferred the following invariants were opened: ") 
-        (pp (add_iname inv_p
-              (remove_iname inv_p inames inv)
-            inv)) ^/^
+        (pp (add_iname
+              (remove_iname inames i)
+            i)) ^/^
       prefix 4 1 (text "But expected to only open: ") (pp inames)
     ]
       
   | Some tok -> tok
 
-module R = FStar.Reflection.V2
+// module R = FStar.Reflection.V2
 
-#push-options "--warn_error -271"
-let tm_star_inj (p1 p2 q:term)
-  : Lemma (requires tm_star p1 q == tm_star p2 q)
-          (ensures p1 == p2) =
-  let aux tv
-    : Lemma (ensures R.inspect_ln (R.pack_ln tv) == tv)
-            [SMTPat ()] = R.inspect_pack_inv tv in
-  ()
-#pop-options
+// #push-options "--warn_error -271"
+// let tm_star_inj (p1 p2 q:term)
+//   : Lemma (requires tm_star p1 q == tm_star p2 q)
+//           (ensures p1 == p2) =
+//   let aux tv
+//     : Lemma (ensures R.inspect_ln (R.pack_ln tv) == tv)
+//             [SMTPat ()] = R.inspect_pack_inv tv in
+//   ()
+// #pop-options
 
-#push-options "--z3rlimit_factor 8 --split_queries no"
+//
+// Find i -~- p in pre, where pre is well-typed
+//
+let rec find_inv (#g:env) (#pre:term) (pre_typing:tot_typing g pre tm_vprop) (i:term)
+  : option (p:term &
+            frame:term &
+            tot_typing g (tm_inv i p) tm_vprop &
+            tot_typing g frame tm_vprop &
+            vprop_equiv g (tm_star (tm_inv i p) frame) pre) =
+
+  match inspect_term pre with
+  | Tm_Inv i' p ->
+    if eq_tm i i'
+    then let frame = tm_emp in
+         let tm_inv_typing = magic () in
+         let frame_typing = magic () in
+         let d_eq = magic () in
+         Some (| p, frame, tm_inv_typing, frame_typing, d_eq |)
+    else None
+  
+  | Tm_Star l r -> begin
+    match find_inv #g #l (magic ()) i with
+    | Some res ->
+      let (| p, frame, _, _, _ |) = res in
+     Some (| p, tm_star frame r, magic (), magic (), magic () |)
+    | None ->
+      match find_inv #g #l (magic ()) i with
+      | Some res ->
+        let (| p, frame, _, _, _ |) = res in
+        Some (| p, tm_star l frame, magic (), magic (), magic () |)
+      | _ -> None
+    end
+    
+  | _ -> None
+
+let find_inv_post (#g:env) (x:var { lookup g x == None})
+  (u:universe)
+  (ret_ty:term)
+  (post:term)
+  (ret_ty_typing:universe_of g ret_ty u)
+  (post_typing:tot_typing (push_binding g x ppname_default ret_ty) (open_term post x) tm_vprop)
+  (i:term)
+
+  : T.Tac (option (p:term &
+                   frame:term &
+                   tot_typing g (tm_inv i p) tm_vprop &
+                   tot_typing (push_binding g x ppname_default ret_ty) (open_term frame x) tm_vprop &
+                   vprop_equiv (push_binding g x ppname_default ret_ty)
+                               (tm_star (tm_inv i p) (open_term frame x))
+                               (open_term post x))) =
+  
+  let post_opened = open_term_nv post (ppname_default, x) in
+  let res = find_inv #_ #post_opened post_typing i in
+  match res with
+  | None -> None
+  | Some (| p, frame, inv_typing, frame_typing, d_eq |) ->
+    let frame_typing : tot_typing _ frame tm_vprop = frame_typing in
+    assume (open_term (close_term frame x) x == frame);
+    let tm_inv_typing : tot_typing g (tm_inv i p) tm_vprop = recheck () in
+    Some (| p, close_term frame x, tm_inv_typing, frame_typing, d_eq |)
+
+// (#pre:term) (pre_typing:tot_typing g pre tm_vprop) (i:term)
+//   : option (p:term &
+//             frame:term &
+//             tot_typing g (tm_inv i p) tm_vprop &
+//             tot_typing g frame tm_vprop &
+//             vprop_equiv g pre (tm_star (tm_inv i p) frame)) =
+
+//   match inspect_term pre with
+//   | Tm_Inv i' p ->
+//     if eq_tm i i'
+//     then let frame = tm_emp in
+//          let tm_inv_typing = magic () in
+//          let frame_typing = magic () in
+//          let d_eq = magic () in
+//          Some (| p, frame, tm_inv_typing, frame_typing, d_eq |)
+//     else None
+  
+//   | Tm_Star l r -> begin
+//     match find_inv_pre #g #l (magic ()) i with
+//     | Some res ->
+//       let (| p, frame, _, _, _ |) = res in
+//      Some (| p, tm_star frame r, magic (), magic (), magic () |)
+//     | None ->
+//       match find_inv_pre #g #l (magic ()) i with
+//       | Some res ->
+//         let (| p, frame, _, _, _ |) = res in
+//         Some (| p, tm_star l frame, magic (), magic (), magic () |)
+//       | _ -> None
+//     end
+    
+//   | _ -> None
+
+#restart-solver
+#push-options "--z3rlimit_factor 10 --split_queries no"
 let check
   (g:env)
   (pre:term)
@@ -193,8 +275,8 @@ let check
   (t:st_term{Tm_WithInv? t.term})
   (check:check_t)
 : T.Tac (checker_result_t g pre post_hint)
-= let Tm_WithInv {name=inv_tm; returns_inv; body} = t.term in
-  let post : post_hint_t =
+= let Tm_WithInv {name=i; returns_inv; body} = t.term in
+  let post_hint : post_hint_t =
     match returns_inv, post_hint with
     | None, Some p -> p
     | Some (b, p), None ->
@@ -208,7 +290,7 @@ let check
     | _, _ ->
       fail g (Some t.range) "Fatal: no post hint on with_invariant"
   in
-  match post.effect_annot with
+  match post_hint.effect_annot with
   | EffectAnnotGhost _ -> 
     let open Pulse.PP in
     fail_doc g (Some t.range) 
@@ -218,131 +300,139 @@ let check
     (* Checking the body seems to change its range, so store the original one
     for better errors. *)
     let body_range = body.range in
-    let inv_tm_range = Pulse.RuntimeUtils.range_of_term inv_tm in
+    let i_range = Pulse.RuntimeUtils.range_of_term i in
 
-    // info_doc g (Some t.range) [
-    //   let open Pulse.PP in
-    //   prefix 4 1 (doc_of_string "Checker.WithInv: using post_hint =") (pp post_hint)
-    // ];
+    let res = find_inv pre_typing i in
+    if None? res then fail g (Some i_range) "Cannot find inv in the context";
+    
+    let Some (| p, pre_frame, inv_typing, pre_frame_typing, d_pre_frame_eq |) = res in
 
-    (* FIXME: should check `inv_tm` at expected type `inv ?u`, and then
-    we obtain vprop from u. If so the whole block below should not be
-    needed. *)
-    let (| inv_tm, eff, inv_tm_ty, inv_tm_typing |) = compute_term_type g inv_tm in
+    let pre_body : vprop = tm_star p pre_frame in
+    //
+    // we know tm_inv i p is well-typed,
+    // so p is well-typed
+    // and frame is well-typed
+    // therefore tm_star is well-typed
+    //
+    let pre_body_typing : tot_typing g pre_body tm_vprop = magic () in
 
-    if eff <> T.E_Total then
-      fail g (Some inv_tm_range) "Ghost effect on inv?";
-
-    (* Check the term without an expected type, and check that it's Tm_Inv p *)
-    let inv_p =
-      match inspect_term inv_tm_ty with
-      | Tm_Inv p -> p
-      | Tm_FStar _ ->
-        fail g (Some inv_tm_range)
-          (Printf.sprintf "Does not have invariant type (%s)" (P.term_to_string inv_tm_ty))
-
-      | _ -> begin
-        (* FIXME: should unrefine... meh *)
-        let ropt = Pulse.Syntax.Pure.is_fvar_app inv_tm_ty in
-        match ropt with
-        | Some (lid, _, _, Some tm) -> 
-          if lid = ["Pulse"; "Lib"; "Core"; "inv" ]
-          then tm
-          else fail g (Some inv_tm_range)
-                    (Printf.sprintf "Does not have invariant type (%s)" (P.term_to_string inv_tm_ty))
-        | _ -> fail g (Some inv_tm_range)
-                    (Printf.sprintf "Does not have invariant type (%s)" (P.term_to_string inv_tm_ty))
-      end
+    let x = fresh g in
+    assume (fresh_wrt x g (freevars post_hint.post));
+    let g' = (push_binding g x ppname_default post_hint.ret_ty) in
+    let post_hint_ret_ty_typing
+      : universe_of g post_hint.ret_ty post_hint.u = recheck () in
+    let post_hint_post_typing
+      : tot_typing g'
+                   (open_term_nv post_hint.post (ppname_default, x))
+                   tm_vprop
+      = recheck ()
     in
     
-    (* FIXME: This is bogus for the wr case!!! *)
-    assume (tm_inv inv_p == inv_tm_ty);
+    let res = find_inv_post #g
+      x
+      post_hint.u
+      post_hint.ret_ty
+      post_hint.post
+      post_hint_ret_ty_typing
+      post_hint_post_typing
+      i in
 
-    (* Can this come from some inversion instead? *)
-    let inv_p_typing : tot_typing g inv_p tm_vprop = recheck () in
+    if None? res then fail g (Some i_range) "Cannot find inv in the postcondition";
 
-    (* pre'/post' are extended with inv_p *)
-    let pre' : vprop = tm_star pre inv_p in
-    let pre'_typing : tot_typing g pre' tm_vprop = recheck () in
+    let Some (| p', post_frame, _, post_frame_typing, d_post_frame_equiv |) = res in
+    assume (p' == p);
 
-    let post_p' : vprop = tm_star post.post inv_p in
-    let elab_ret_ty = elab_term post.ret_ty in
-    let x = fresh g in
-    assume (fresh_wrt x g (freevars post_p'));
-    // Pulse.Typing.FV.freevars_close_term post_p' x 0;
-    // let post_p' = close_term post_p' x in
-    let g' = (push_binding g x ppname_default post.ret_ty) in
-    let r_g' = elab_env g' in
-    let post_p'_typing_src
-      : RT.tot_typing r_g'
-                      (elab_term (open_term_nv post_p' (v_as_nv x)))
-                      (elab_term tm_vprop)
-      = rt_recheck g' #r_g' ()
-    in
-    let post_p'_typing = Pulse.Checker.Base.post_typing_as_abstraction #g #_ #post.ret_ty #post_p' (E post_p'_typing_src) in
-    (* the post hint for the body, extended with inv_p, removing the name of invariant *)
-  begin
+    let post_body = tm_star p post_frame in
+    
     let (| opens, opens_typing |) 
       : t:term & tot_typing g t tm_inames 
-      = match post.effect_annot with
+      = match post_hint.effect_annot with
         | EffectAnnotSTT ->
           (| all_inames, all_inames_typing g |)
         | EffectAnnotAtomic { opens } ->
-          (| opens, (post_hint_typing g post x).effect_annot_typing |)
+          (| opens, (post_hint_typing g post_hint x).effect_annot_typing |)
     in
-    let opens_remove_i = remove_iname inv_p opens inv_tm in
+    let opens_remove_i = remove_iname opens i in
     let effect_annot = EffectAnnotAtomic { opens=opens_remove_i } in
     let effect_annot_typing
       : effect_annot_typing g effect_annot
-      = remove_iname_typing g #inv_p #opens #inv_tm inv_p_typing opens_typing inv_tm_typing
+      = remove_iname_typing g #opens #i opens_typing (magic ())  // from inversion of tm_inv_typing
     in
-    let post' : post_hint_for_env g =  { post with
+
+    assume (fresh_wrt x g (freevars post_body));
+    let post_hint_body : post_hint_for_env g =  { post_hint with
       effect_annot;
       effect_annot_typing;
       g;
-      ty_typing = recheck (); // Pulse.Typing.Metatheory.tot_typing_weakening _ _ _ _ post.ty_typing _;
-      post = post_p';
+      ty_typing = post_hint_ret_ty_typing;
+      post = post_body;
       x;
-      post_typing_src=E post_p'_typing_src;
-      post_typing = post_p'_typing;
+      post_typing_src=magic ();
+      post_typing=magic ();
     } in
+
     let (| body, c_body, body_typing |) =
       let ppname = mk_ppname_no_range "with_inv_body" in
-      let r = check g pre' pre'_typing (Some post') ppname body in
+      let r = check g pre_body pre_body_typing (Some post_hint_body) ppname body in
       apply_checker_result_k r ppname
     in
+
     let C_STAtomic inames obs st = c_body in
     assert (inames == opens_remove_i);
-    let c_out = C_STAtomic inames obs (st_comp_remove_inv inv_p st) in
-    assert (tm_star (comp_pre c_out) inv_p == pre');
-    tm_star_inj (comp_pre c_out) pre inv_p;
-    assert (comp_pre c_out == pre);
-    assert (add_inv c_out inv_p == c_body);
-    let tok = disjointness_remove_i_i g inv_p opens inv_tm in
-    let tm : st_term =
-      { term = Tm_WithInv {name=inv_tm; body; returns_inv = None};
-        range = t.range;
-        effect_tag = Sealed.seal (Some <| ctag_of_effect_annot post.effect_annot) }
+    assert (st.pre == tm_star p pre_frame);
+    assert (st.post == tm_star p post_frame);
+
+    let c_out = C_STAtomic (Pulse.Reflection.Util.add_inv_tm inames i) obs
+      {st with pre = pre;
+       post = post_hint.post} in
+
+    let tok = disjointness_remove_i_i g opens i in
+    let d : st_typing _ _ c_out =
+      let c = C_STAtomic inames obs { st with pre = pre_frame; post = post_frame  } in
+      let c_out_eq = C_STAtomic (Pulse.Reflection.Util.add_inv_tm inames i) obs
+        {st with pre = tm_star (tm_inv i p ) pre_frame;
+         post = tm_star (tm_inv i p) post_frame} in
+      assert (add_frame_l c p == c_body);
+      assert (comp_with_inv_atomic c i p == c_out_eq);
+      let d : st_typing _ _ c_out_eq =
+        T_WithInv _ i p _ c (magic ()) (magic ()) body_typing tok in
+      let d_pre_eq : vprop_equiv g (comp_pre c_out_eq) (comp_pre c_out) = d_pre_frame_eq in
+      let d_post_eq : vprop_equiv (push_binding g x ppname_default post_hint.ret_ty)
+                                  (tm_star (tm_inv i p) (open_term post_frame x))
+                                  (open_term post_hint.post x) = d_post_frame_equiv in
+      assume (open_term (tm_inv i p) x == tm_inv i p);
+      assert (comp_post c_out_eq == tm_star (tm_inv i p) post_frame);
+      assume (open_term (comp_post c_out_eq) x ==
+              tm_star (tm_inv i p) (open_term post_frame x));
+      let d_post_eq : vprop_equiv (push_binding g x ppname_default post_hint.ret_ty)
+                                  (open_term (comp_post c_out_eq) x)
+                                  (open_term (comp_post c_out) x) = d_post_eq in
+      assert (comp_res c_out_eq == comp_res c_out);
+      assume (~ (x `Set.mem` freevars (comp_post c_out_eq)));
+      assume (~ (x `Set.mem` freevars (comp_post c_out)));
+      T_Equiv _ _ _ _ d
+        (ST_VPropEquiv _ c_out_eq c_out x (magic ())
+                                          (magic ())
+                                          (magic ())
+                                          (RT.Rel_refl _ _ RT.R_Eq)
+                                          d_pre_eq
+                                          d_post_eq)
     in
-      
-    let d = T_WithInv g inv_tm inv_p inv_p_typing inv_tm_typing body c_out body_typing tok in
-    let c_out = add_iname_at_least_unobservable c_out inv_p inv_tm in
-    let d : st_typing _ _ c_out = d in
-    match post.effect_annot with
+
+    match post_hint.effect_annot with
     | EffectAnnotAtomic _ -> 
-      let C_STAtomic add_inv obs' st = c_out in
+      let C_STAtomic add_inv obs st = c_out in
       let tok : prop_validity g (tm_inames_subset add_inv opens) =
-        add_remove_inverse g inv_p opens inv_tm
-            inv_p_typing
+        add_remove_inverse g opens i
             opens_typing
-            inv_tm_typing
+            (magic ())
       in
-      let c_out = C_STAtomic opens obs' st in
+      let c_out = C_STAtomic opens obs st in
       let d : st_typing _ _ c_out =
-        T_Sub _ _ _ _ d (STS_AtomicInvs _ st add_inv opens obs' obs' tok) in
-      checker_result_for_st_typing (| tm, _, d |) res_ppname
+        T_Sub _ _ _ _ d (STS_AtomicInvs _ st add_inv opens obs obs tok) in
+      checker_result_for_st_typing (| _, _, d |) res_ppname
+
     | EffectAnnotSTT ->
       let d = T_Lift _ _ _ _ d (Lift_STAtomic_ST _ c_out) in
-      checker_result_for_st_typing (| tm, _, d |) res_ppname
-    end
+      checker_result_for_st_typing (| _, _, d |) res_ppname
 #pop-options
