pulse/src/checker/Pulse.Reflection.Util.fst
@@ -43,6 +43,7 @@ let reveal_lid = ["FStar"; "Ghost"; "reveal"]
 let vprop_lid = mk_pulse_lib_core_lid "vprop"
 let vprop_fv = R.pack_fv vprop_lid
 let vprop_tm = R.pack_ln (R.Tv_FVar vprop_fv)
+let emp_lid = mk_pulse_lib_core_lid "emp"
 let unit_fv = R.pack_fv unit_lid
 let unit_tm = R.pack_ln (R.Tv_FVar unit_fv)
 let bool_fv = R.pack_fv bool_lid
@@ -91,10 +92,6 @@ let mk_snd (u1 u2:R.universe) (a1 a2 e:R.term) : R.term =
 
 let true_tm = R.pack_ln (R.Tv_Const (R.C_True))
 let false_tm = R.pack_ln (R.Tv_Const (R.C_False))
-
-let inv_lid = mk_pulse_lib_core_lid "inv"
-let emp_lid = mk_pulse_lib_core_lid "emp"
-let inames_lid = mk_pulse_lib_core_lid "inames"
 
 let star_lid = mk_pulse_lib_core_lid "op_Star_Star"
 
@@ -160,10 +157,6 @@ let mk_stt_ghost_admit (u:R.universe) (t pre post:R.term) : R.term =
   let t = pack_ln (Tv_App t (pre, Q_Explicit)) in
   pack_ln (Tv_App t (post, Q_Explicit))
 
-let emp_inames_lid = mk_pulse_lib_core_lid "emp_inames"
-let all_inames_lid = mk_pulse_lib_core_lid "all_inames"
-let add_inv_lid = mk_pulse_lib_core_lid "add_inv"
-let remove_inv_lid = mk_pulse_lib_core_lid "remove_inv"
 let elim_pure_lid = mk_pulse_lib_core_lid "elim_pure"
 
  //the thunked, value-type counterpart of the effect STT
@@ -294,17 +287,6 @@ let vprop_eq_tm t1 t2 =
   let t = pack_ln (Tv_App t (t1, Q_Explicit)) in
   let t = pack_ln (Tv_App t (t2, Q_Explicit)) in
   t
-
-let emp_inames_tm : R.term = R.pack_ln (R.Tv_FVar (R.pack_fv emp_inames_lid))
-let all_inames_tm : R.term = R.pack_ln (R.Tv_FVar (R.pack_fv all_inames_lid))
-
-let add_inv_tm (p is i : R.term) : R.term =
-  let h = R.pack_ln (R.Tv_FVar (R.pack_fv add_inv_lid)) in
-  R.mk_app h [im p; ex is; ex i]
-
-let remove_inv_tm (p is i : R.term) : R.term =
-  let h = R.pack_ln (R.Tv_FVar (R.pack_fv remove_inv_lid)) in
-  R.mk_app h [im p; ex is; ex i]
 
 let non_informative_lid = mk_pulse_lib_noninformative_lid "non_informative"
 let non_informative_rt (u:R.universe) (a:R.term) : R.term =
@@ -743,18 +725,31 @@ let mk_opaque_let (g:R.env) (nm:string) (tm:Ghost.erased R.term) (ty:R.typ{RT.ty
   in
   (true, se, None)
 
-let mk_mem_inv (invP inames inv:R.term) : R.term =
-  let mem_inv_tm = mk_pulse_lib_core_lid "mem_inv" in
-  let t = R.pack_ln (R.Tv_FVar (R.pack_fv mem_inv_tm)) in
-  R.mk_app t [ im invP; ex inames; ex inv ]
-
-let inv_disjointness_goal (inv_p:T.term) (inames:T.term) (inv:T.term) 
-: R.term 
-= let p = mk_mem_inv inv_p inames inv in
-  let u0 = R.pack_universe R.Uv_Zero in
-  let p = mk_reveal u0 bool_tm p in
-  mk_eq2 u0 bool_tm (`false) p
-
 let mk_observability_lid l = ["PulseCore"; "Observability"; l]
 let observable_lid = mk_observability_lid "Observable"
 let neutral_lid = mk_observability_lid "Neutral"
+
+let inames_lid = mk_pulse_lib_core_lid "inames"
+let iname_ref_lid = mk_pulse_lib_core_lid "iname_ref"
+let inv_lid = mk_pulse_lib_core_lid "op_Subtraction_Tilde_Subtraction"
+let emp_inames_lid = mk_pulse_lib_core_lid "emp_inames"
+let all_inames_lid = mk_pulse_lib_core_lid "all_inames"
+let add_inv_lid = mk_pulse_lib_core_lid "add_inv"
+let remove_inv_lid = mk_pulse_lib_core_lid "remove_inv"
+
+let add_inv_tm (is iref:R.term) : R.term =
+  let h = R.pack_ln (R.Tv_FVar (R.pack_fv add_inv_lid)) in
+  R.mk_app h [ex is; ex iref]
+let remove_inv_tm (is iref:R.term) : R.term =
+  let h = R.pack_ln (R.Tv_FVar (R.pack_fv remove_inv_lid)) in
+  R.mk_app h [ex is; ex iref]
+let mk_mem_inv (is iref:R.term) : R.term =
+  let mem_inv_tm = mk_pulse_lib_core_lid "mem_inv" in
+  let t = R.pack_ln (R.Tv_FVar (R.pack_fv mem_inv_tm)) in
+  R.mk_app t [ ex is; ex iref ]
+
+let inv_disjointness_goal (is iref:R.term) : R.term =
+  let p = mk_mem_inv is iref in
+  let u0 = R.pack_universe R.Uv_Zero in
+  let p = mk_reveal u0 bool_tm p in
+  mk_eq2 u0 bool_tm (`false) p
