pulse/src/checker/Pulse.Syntax.Printer.fst
@@ -113,13 +113,10 @@ and term_to_string' (level:string) (t:term) : T.Tac string
     | Tm_Inames -> "inames"
     | Tm_EmpInames -> "emp_inames"
     | Tm_Unknown -> "_"
-    | Tm_AddInv i is ->
-      sprintf "add_inv %s %s"
+    | Tm_Inv i p ->
+      sprintf "%s -~- %s"
         (term_to_string' level i)
-        (term_to_string' level is)
-    | Tm_Inv i ->
-      sprintf "inv %s"
-        (term_to_string' level i)
+        (term_to_string' level p)
     | Tm_FStar t -> T.term_to_string t
 
 let term_to_string t = term_to_string' "" t
@@ -154,10 +151,11 @@ and term_to_doc t : T.Tac document
     | Tm_VProp -> doc_of_string "vprop"
     | Tm_Inames -> doc_of_string "inames"
     | Tm_EmpInames -> doc_of_string "emp_inames"
-    | Tm_AddInv i is ->
-      doc_of_string "add_inv" ^/^ parens (term_to_doc i ^^ doc_of_string "," ^^ term_to_doc is)
-    | Tm_Inv i ->
-      doc_of_string "inv" ^/^ parens (term_to_doc i)
+    | Tm_Inv i p ->
+      infix 2 1 (doc_of_string "-~-")
+                (term_to_doc i)
+                (term_to_doc p)
+
     | Tm_Unknown -> doc_of_string "_"
     | Tm_FStar t -> doc_of_string (T.term_to_string t) 
 
@@ -438,8 +436,7 @@ let tag_of_term (t:term) =
   | Tm_Inames -> "Tm_Inames"
   | Tm_EmpInames -> "Tm_EmpInames"
   | Tm_Unknown -> "Tm_Unknown"
-  | Tm_AddInv _ _ -> "Tm_AddInv"
-  | Tm_Inv _ -> "Tm_Inv"
+  | Tm_Inv _ _ -> "Tm_Inv"
   | Tm_FStar _ -> "Tm_FStar"
 
 let tag_of_st_term (t:st_term) =
